@prefix : <http://www.semanticweb.org/superjordi/ontologies/2024/3/travel-experience-ontology/> .
@prefix owl: <http://www.w3.org/2002/07/owl#> .
@prefix rdf: <http://www.w3.org/1999/02/22-rdf-syntax-ns#> .
@prefix xml: <http://www.w3.org/XML/1998/namespace> .
@prefix xsd: <http://www.w3.org/2001/XMLSchema#> .
@prefix rdfs: <http://www.w3.org/2000/01/rdf-schema#> .
@base <http://www.semanticweb.org/superjordi/ontologies/2024/3/travel-experience-ontology/> .

<http://www.semanticweb.org/superjordi/ontologies/2024/3/travel-experience-ontology> rdf:type owl:Ontology .

#################################################################
#    Annotation properties
#################################################################

###  http://www.w3.org/2000/01/rdf-schema#label
rdfs:label rdfs:comment "Indicates the flights that are operated by an airline, connecting airline companies with the specific flights they manage." .


#################################################################
#    Object Properties
#################################################################

###  http://www.semanticweb.org/superjordi/ontologies/2024/3/travel-experience-ontology#booksSeat
:booksSeat rdf:type owl:ObjectProperty ;
           rdfs:domain :Passenger ;
           rdfs:range :Seat ;
           rdfs:comment "Links a passenger to the seat they have booked." ;
           rdfs:label "Books Seat" .


###  http://www.semanticweb.org/superjordi/ontologies/2024/3/travel-experience-ontology/arrivalFor
:arrivalFor rdf:type owl:ObjectProperty .


###  http://www.semanticweb.org/superjordi/ontologies/2024/3/travel-experience-ontology/arriveAt
:arriveAt rdf:type owl:ObjectProperty ,
                   owl:FunctionalProperty ;
          rdfs:domain :Flight ;
          rdfs:range :Airport ;
          rdfs:comment "Denotes the airport where the flight will land, completing its journey." ;
          rdfs:label "arrives at" .


###  http://www.semanticweb.org/superjordi/ontologies/2024/3/travel-experience-ontology/departFrom
:departFrom rdf:type owl:ObjectProperty ;
            owl:inverseOf :departureFor ;
            rdf:type owl:FunctionalProperty ;
            rdfs:domain :Flight ;
            rdfs:range :Airport ;
            rdfs:comment "Specifies the airport from which a particular flight departs." ;
            rdfs:label "departs from" .


###  http://www.semanticweb.org/superjordi/ontologies/2024/3/travel-experience-ontology/departureFor
:departureFor rdf:type owl:ObjectProperty .


###  http://www.semanticweb.org/superjordi/ontologies/2024/3/travel-experience-ontology/hasPassenger
:hasPassenger rdf:type owl:ObjectProperty ;
              owl:inverseOf :isPassengerOn ;
              rdfs:domain :Flight ;
              rdfs:range :Passenger ;
              rdfs:comment "Connects a flight to its passengers, representing those who are traveling on a specific flight." ;
              rdfs:label "has passenger" .


###  http://www.semanticweb.org/superjordi/ontologies/2024/3/travel-experience-ontology/isOperatedBy
:isOperatedBy rdf:type owl:ObjectProperty ;
              owl:inverseOf :operatesFlight .


###  http://www.semanticweb.org/superjordi/ontologies/2024/3/travel-experience-ontology/isPassengerOn
:isPassengerOn rdf:type owl:ObjectProperty .


###  http://www.semanticweb.org/superjordi/ontologies/2024/3/travel-experience-ontology/operatesFlight
:operatesFlight rdf:type owl:ObjectProperty ;
                rdfs:domain :Airline ;
                rdfs:range :Flight ;
                rdfs:comment "Indicates the flights that are operated by an airline, connecting airline companies with the specific flights they manage." ;
                rdfs:label "operates flight" .


#################################################################
#    Data properties
#################################################################

###  http://www.semanticweb.org/superjordi/ontologies/2024/3/travel-experience-ontology/flightDuration
:flightDuration rdf:type owl:DatatypeProperty ,
                         owl:FunctionalProperty ;
                rdfs:domain :Flight ;
                rdfs:range xsd:dateTime ;
                rdfs:comment "Indicates the total duration of the flight, typically expressed in ISO 8601 duration format." ;
                rdfs:label "flight duration" .


###  http://www.semanticweb.org/superjordi/ontologies/2024/3/travel-experience-ontology/numberOfFlights
:numberOfFlights rdf:type owl:DatatypeProperty ,
                          owl:FunctionalProperty ;
                 rdfs:domain :Passenger ;
                 rdfs:range xsd:integer ;
                 rdfs:comment "Counts how many flights the passenger has taken, useful for frequent flyer tracking and benefits." ;
                 rdfs:label "number of flights" .


###  http://www.semanticweb.org/superjordi/ontologies/2024/3/travel-experience-ontology/overallRating
:overallRating rdf:type owl:DatatypeProperty ,
                        owl:FunctionalProperty ;
               rdfs:domain :Review ;
               rdfs:range xsd:float ;
               rdfs:comment "Represents the overall satisfaction rating given by a passenger in their review, typically on a scale from 1 to 10." ;
               rdfs:label "overall rating" .


###  http://www.semanticweb.org/superjordi/ontologies/2024/3/travel-experience-ontology/reviewDate
:reviewDate rdf:type owl:DatatypeProperty ,
                     owl:FunctionalProperty ;
            rdfs:domain :Review ;
            rdfs:range xsd:dateTime ;
            rdfs:comment "Specifies the date on which the review was published by the passenger." ;
            rdfs:label "review date" .


###  http://www.semanticweb.org/superjordi/ontologies/2024/3/travel-experience-ontology/seatComfortRating
:seatComfortRating rdf:type owl:DatatypeProperty ,
                            owl:FunctionalProperty ;
                   rdfs:domain :SeatReview ;
                   rdfs:range xsd:integer ;
                   rdfs:comment "Provides a numerical rating for the comfort of the seat as reviewed by the passenger, on a scale typically from 1 to 5." ;
                   rdfs:label "seat comfort rating" .


#################################################################
#    Classes
#################################################################

###  http://www.semanticweb.org/superjordi/ontologies/2024/3/travel-experience-ontology/Airline
:Airline rdf:type owl:Class ;
         rdfs:subClassOf :TravelExperience .


###  http://www.semanticweb.org/superjordi/ontologies/2024/3/travel-experience-ontology/Airport
:Airport rdf:type owl:Class ;
         rdfs:subClassOf :TravelExperience .


###  http://www.semanticweb.org/superjordi/ontologies/2024/3/travel-experience-ontology/BaggageService
:BaggageService rdf:type owl:Class ;
                rdfs:subClassOf :GroundService ;
                rdfs:comment "Services related to handling passenger luggage before and after the flight." ;
                rdfs:label "Baggage Service" .


###  http://www.semanticweb.org/superjordi/ontologies/2024/3/travel-experience-ontology/Business
:Business rdf:type owl:Class ;
          rdfs:subClassOf :TravelClass ;
          rdfs:comment "A class of travel offering more amenities and space than economy class." ;
          rdfs:label "Business Class" .


###  http://www.semanticweb.org/superjordi/ontologies/2024/3/travel-experience-ontology/BusinessClassSeat
:BusinessClassSeat rdf:type owl:Class ;
                   rdfs:subClassOf :Seat ;
                   rdfs:comment "A more spacious and comfortable seat compared to economy, usually with additional services." ;
                   rdfs:label "Business Class Seat" .


###  http://www.semanticweb.org/superjordi/ontologies/2024/3/travel-experience-ontology/CheckInService
:CheckInService rdf:type owl:Class ;
                rdfs:subClassOf :GroundService ;
                rdfs:comment "Services provided during the check-in process before the flight." ;
                rdfs:label "Check-In Service" .


###  http://www.semanticweb.org/superjordi/ontologies/2024/3/travel-experience-ontology/CrewMember
:CrewMember rdf:type owl:Class ;
            rdfs:subClassOf :Person .


###  http://www.semanticweb.org/superjordi/ontologies/2024/3/travel-experience-ontology/CrewReview
:CrewReview rdf:type owl:Class ;
            rdfs:subClassOf :Review ;
            rdfs:comment "A review that assesses the service provided by the flight's crew members." ;
            rdfs:label "Crew Review" .


###  http://www.semanticweb.org/superjordi/ontologies/2024/3/travel-experience-ontology/DomesticAirline
:DomesticAirline rdf:type owl:Class ;
                 rdfs:subClassOf :Airline ;
                 rdfs:comment "An airline operating within a single country, offering domestic flights." ;
                 rdfs:label "Domestic Airline" .


###  http://www.semanticweb.org/superjordi/ontologies/2024/3/travel-experience-ontology/Economy
:Economy rdf:type owl:Class ;
         rdfs:subClassOf :TravelClass ;
         rdfs:label "Economy Class" ,
                    "The most common and affordable class of travel on commercial flights." .


###  http://www.semanticweb.org/superjordi/ontologies/2024/3/travel-experience-ontology/EconomyClassSeat
:EconomyClassSeat rdf:type owl:Class ;
                  rdfs:subClassOf :Seat ;
                  rdfs:comment "A seat in the economy class, typically offering basic amenities." ;
                  rdfs:label "Economy Class Seat" .


###  http://www.semanticweb.org/superjordi/ontologies/2024/3/travel-experience-ontology/Entertainment
:Entertainment rdf:type owl:Class ;
               rdfs:subClassOf :InFlightService ;
               rdfs:comment "Entertainment options available to passengers during the flight such as movies, music, and games." ;
               rdfs:label "In-Flight Entertainment" .


###  http://www.semanticweb.org/superjordi/ontologies/2024/3/travel-experience-ontology/FirstClass
:FirstClass rdf:type owl:Class ;
            rdfs:subClassOf :TravelClass ;
            rdfs:comment "The highest class of travel with the most amenities and services offered." ;
            rdfs:label "First Class" .


###  http://www.semanticweb.org/superjordi/ontologies/2024/3/travel-experience-ontology/FirstClassSeat
:FirstClassSeat rdf:type owl:Class ;
                rdfs:subClassOf :Seat ;
                rdfs:comment "The most luxurious and spacious seat available, with premium services." ;
                rdfs:label "First Class Seat" .


###  http://www.semanticweb.org/superjordi/ontologies/2024/3/travel-experience-ontology/FirstTimeFlyer
:FirstTimeFlyer rdf:type owl:Class ;
                rdfs:subClassOf :Passenger ;
                rdfs:comment "A passenger who is traveling by air for the first time." ;
                rdfs:label "First Time Flyer" .


###  http://www.semanticweb.org/superjordi/ontologies/2024/3/travel-experience-ontology/Flight
:Flight rdf:type owl:Class ;
        rdfs:subClassOf :TravelExperience ,
                        [ rdf:type owl:Restriction ;
                          owl:onProperty :arriveAt ;
                          owl:someValuesFrom :Airport
                        ] ,
                        [ rdf:type owl:Restriction ;
                          owl:onProperty :departFrom ;
                          owl:someValuesFrom :Airport
                        ] ;
        rdfs:comment "Every flight must have a specified departure and arrival airport, which are essential for defining the flight's route." .


###  http://www.semanticweb.org/superjordi/ontologies/2024/3/travel-experience-ontology/FlightAttendant
:FlightAttendant rdf:type owl:Class ;
                 rdfs:subClassOf :CrewMember ;
                 rdfs:comment "A crew member who ensures the safety and comfort of passengers onboard." ;
                 rdfs:label "Flight Attendant" .


###  http://www.semanticweb.org/superjordi/ontologies/2024/3/travel-experience-ontology/FlightLeg
:FlightLeg rdf:type owl:Class ;
           rdfs:subClassOf :TravelExperience ;
           rdfs:comment "Represents one segment of a trip to cases where multiple flights are needed to reach a destination." ;
           rdfs:label "Flight Leg" .


###  http://www.semanticweb.org/superjordi/ontologies/2024/3/travel-experience-ontology/FrequentFlyer
:FrequentFlyer rdf:type owl:Class ;
               rdfs:subClassOf :Passenger ;
               rdfs:comment "A passenger who travels frequently, often accruing miles or benefits." ;
               rdfs:label "Frequent Flyer" .


###  http://www.semanticweb.org/superjordi/ontologies/2024/3/travel-experience-ontology/GroundService
:GroundService rdf:type owl:Class ;
               rdfs:subClassOf :Service .


###  http://www.semanticweb.org/superjordi/ontologies/2024/3/travel-experience-ontology/InFlightService
:InFlightService rdf:type owl:Class ;
                 rdfs:subClassOf :Service .


###  http://www.semanticweb.org/superjordi/ontologies/2024/3/travel-experience-ontology/InternationalAirline
:InternationalAirline rdf:type owl:Class ;
                      rdfs:subClassOf :Airline ;
                      rdfs:comment "An airline offering international flights between multiple countries." ;
                      rdfs:label "International Airline" .


###  http://www.semanticweb.org/superjordi/ontologies/2024/3/travel-experience-ontology/InternationalAirport
:InternationalAirport rdf:type owl:Class ;
                      rdfs:subClassOf :Airport ;
                      rdfs:comment "An airport that serves international flights, potentially a hub for multiple airlines." ;
                      rdfs:label "International Airport" .


###  http://www.semanticweb.org/superjordi/ontologies/2024/3/travel-experience-ontology/Itinerary
:Itinerary rdf:type owl:Class ;
           rdfs:subClassOf :TravelExperience .


###  http://www.semanticweb.org/superjordi/ontologies/2024/3/travel-experience-ontology/LongHaulFlight
:LongHaulFlight rdf:type owl:Class ;
                rdfs:subClassOf :Flight ;
                rdfs:comment "A flight that covers long distances, typically international or intercontinental." ;
                rdfs:label "Long Haul Flight" .


###  http://www.semanticweb.org/superjordi/ontologies/2024/3/travel-experience-ontology/MealReview
:MealReview rdf:type owl:Class ;
            rdfs:subClassOf :Review ;
            rdfs:comment "A review that evaluates the quality and variety of meals provided on the flight." ;
            rdfs:label "Meal Review" .


###  http://www.semanticweb.org/superjordi/ontologies/2024/3/travel-experience-ontology/MealService
:MealService rdf:type owl:Class ;
             rdfs:subClassOf :InFlightService .


###  http://www.semanticweb.org/superjordi/ontologies/2024/3/travel-experience-ontology/MultiFlightItinerary
:MultiFlightItinerary rdf:type owl:Class ;
                      rdfs:subClassOf :Itinerary ;
                      rdfs:comment "An itinerary that includes multiple flight legs to reach the destination." ;
                      rdfs:label "Multi Flight Itinerary" .


###  http://www.semanticweb.org/superjordi/ontologies/2024/3/travel-experience-ontology/OneWayTicket
:OneWayTicket rdf:type owl:Class ;
              rdfs:subClassOf :Ticket ;
              rdfs:comment "A ticket that allows travel from an origin to a destination without a return." ;
              rdfs:label "One-Way Ticket" .


###  http://www.semanticweb.org/superjordi/ontologies/2024/3/travel-experience-ontology/Passenger
:Passenger rdf:type owl:Class ;
           rdfs:subClassOf :Person ,
                           [ rdf:type owl:Restriction ;
                             owl:onProperty :booksSeat ;
                             owl:maxQualifiedCardinality "1"^^xsd:nonNegativeInteger ;
                             owl:onClass :Seat
                           ] .


###  http://www.semanticweb.org/superjordi/ontologies/2024/3/travel-experience-ontology/Person
:Person rdf:type owl:Class ;
        rdfs:subClassOf :TravelExperience .


###  http://www.semanticweb.org/superjordi/ontologies/2024/3/travel-experience-ontology/Pilot
:Pilot rdf:type owl:Class ;
       rdfs:subClassOf :CrewMember ;
       rdfs:comment "A trained professional responsible for flying the aircraft." ;
       rdfs:label "Pilot" .


###  http://www.semanticweb.org/superjordi/ontologies/2024/3/travel-experience-ontology/RegionalAirport
:RegionalAirport rdf:type owl:Class ;
                 rdfs:subClassOf :Airport ;
                 rdfs:comment "An airport serving regional or domestic flights, with fewer international connections." ;
                 rdfs:label "Regional Airport" .


###  http://www.semanticweb.org/superjordi/ontologies/2024/3/travel-experience-ontology/Review
:Review rdf:type owl:Class ;
        rdfs:subClassOf :TravelExperience .


###  http://www.semanticweb.org/superjordi/ontologies/2024/3/travel-experience-ontology/RoundTripTicket
:RoundTripTicket rdf:type owl:Class ;
                 rdfs:subClassOf :Ticket ;
                 rdfs:comment "A ticket that includes both a departure and a return flight." ;
                 rdfs:label "Round Trip Ticket" .


###  http://www.semanticweb.org/superjordi/ontologies/2024/3/travel-experience-ontology/Seat
:Seat rdf:type owl:Class ;
      rdfs:subClassOf :TravelExperience .


###  http://www.semanticweb.org/superjordi/ontologies/2024/3/travel-experience-ontology/SeatReview
:SeatReview rdf:type owl:Class ;
            rdfs:subClassOf :Review ;
            rdfs:comment "A review that focuses specifically on the seating arrangements and comfort." ;
            rdfs:label "Seat Review" .


###  http://www.semanticweb.org/superjordi/ontologies/2024/3/travel-experience-ontology/Service
:Service rdf:type owl:Class ;
         rdfs:subClassOf :TravelExperience .


###  http://www.semanticweb.org/superjordi/ontologies/2024/3/travel-experience-ontology/ShortHaulFlight
:ShortHaulFlight rdf:type owl:Class ;
                 rdfs:subClassOf :Flight ;
                 rdfs:comment "A flight covering a short distance, typically within the same continent." ;
                 rdfs:label "Short Haul Flight" .


###  http://www.semanticweb.org/superjordi/ontologies/2024/3/travel-experience-ontology/SingleFlightItinerary
:SingleFlightItinerary rdf:type owl:Class ;
                       rdfs:subClassOf :Itinerary ;
                       rdfs:comment "An itinerary consisting of a single flight from origin to destination." ;
                       rdfs:label "Single Flight Itinerary" .


###  http://www.semanticweb.org/superjordi/ontologies/2024/3/travel-experience-ontology/SpecialMeal
:SpecialMeal rdf:type owl:Class ;
             rdfs:subClassOf :MealService ;
             rdfs:comment "A meal option catering to specific dietary requirements or preferences." ;
             rdfs:label "Special Meal" .


###  http://www.semanticweb.org/superjordi/ontologies/2024/3/travel-experience-ontology/StandardMeal
:StandardMeal rdf:type owl:Class ;
              rdfs:subClassOf :MealService ;
              rdfs:comment "The regular meal option provided to all passengers." ;
              rdfs:label "Standard Meal" .


###  http://www.semanticweb.org/superjordi/ontologies/2024/3/travel-experience-ontology/Ticket
:Ticket rdf:type owl:Class ;
        rdfs:subClassOf :TravelExperience .


###  http://www.semanticweb.org/superjordi/ontologies/2024/3/travel-experience-ontology/TravelClass
:TravelClass rdf:type owl:Class ;
             rdfs:subClassOf :TravelExperience .


###  http://www.semanticweb.org/superjordi/ontologies/2024/3/travel-experience-ontology/TravelExperience
:TravelExperience rdf:type owl:Class .


###  Generated by the OWL API (version 4.5.26.2023-07-17T20:34:13Z) https://github.com/owlcs/owlapi
